books/kestrel/crypto/blake/blake2s-extended.lisp
@@ -1,6 +1,6 @@
 ; A variant of blake2s that supports a salt input and a personalization input
 ;
-; Copyright (C) 2021 Kestrel Institute
+; Copyright (C) 2021-2025 Kestrel Institute
 ;
 ; License: A 3-clause BSD license. See the file books/3BSD-mod.txt.
 ;
@@ -32,6 +32,7 @@
 (local (include-book "kestrel/lists-light/append" :dir :system))
 (local (include-book "kestrel/lists-light/take" :dir :system))
 (local (include-book "kestrel/lists-light/len" :dir :system))
+(local (include-book "kestrel/lists-light/nth" :dir :system))
 (local (include-book "kestrel/arithmetic-light/mod-and-expt" :dir :system))
 (local (include-book "kestrel/arithmetic-light/ceiling" :dir :system))
 (local (include-book "kestrel/arithmetic-light/floor" :dir :system))
@@ -103,53 +104,7 @@
          (len words1))
   :hints (("Goal" :in-theory (enable xor-words))))
 
-; Matt K. mod 7/31/2023 to accommodate evaluation inside lambda bodies when
-; generating guard conjectures.
-(local (in-theory (disable (:e expt))))
-
-;; This function replaces the function blake2s-main.
-;;TODO: Consider the case when ll is the max.  Then (+ ll *bb*) is > 2^64, contrary to the documentation of f.
-(defund blake2s-extended-main (d ll kk nn parameter-block)
-  (declare (xargs :guard (and (true-listp d)
-                              (all-blockp d)
-                              (< 0 (len d))
-                              (<= (len d) (/ *blake2s-max-data-byte-length* 64)) ;think about this
-                              (natp ll)
-                              ;; (< ll (- *blake2s-max-data-byte-length* 64))
-                              (< ll *blake2s-max-data-byte-length*)
-                              (natp kk)
-                              (posp nn)
-                              (<= nn 32)
-                              (true-listp parameter-block)
-                              (all-wordp parameter-block)
-                              (equal (len parameter-block) 8))
-                  :guard-hints (("Goal" :expand ((wordp nn)
-                                                 (unsigned-byte-p 64 (+ 64 ll)))
-                                 :in-theory (e/d (natp) ())))))
-  (let* ((h (xor-words (iv) parameter-block)) ; this is what differs from the version in blake2s.lisp
-         (dd (len d))
-         (h (if (> dd 1)
-                (loop1 0 (- dd 2) h d)
-              h))
-         (h (if (= kk 0)
-                (f h (nth (- dd 1) d) ll t)
-              (f h
-                 (nth (- dd 1) d)
-                 (mod (+ ll *bb*) (expt 2 (* 2 *w*)))
-                 t))))
-    (take nn (words-to-bytes h))))
-
-(defthm len-of-blake2s-extended-main
-  (implies (and (posp nn)
-                (<= nn 32))
-           (equal (len (blake2s-extended-main d ll kk nn parameter-block))
-                  nn))
-  :hints (("Goal" :in-theory (enable blake2s-extended-main))))
-
-(defthm all-unsigned-byte-p-of-blake2s-extended-main
-  (implies (<= nn 32)
-           (all-unsigned-byte-p 8 (blake2s-extended-main d ll kk nn parameter-block)))
-  :hints (("Goal" :in-theory (enable blake2s-extended-main))))
+;;;;;;;;;;;;;;;;;;;;;;;;;;;;;;;;;;;;;;;;;;;;;;;;;;;;;;;;;;;;;;;;;;;;;;;;;;;;;;;;
 
 ;; This function replaces the function blake2s.
 ;; Returns the hash, as a list of bytes of length NN.
@@ -160,19 +115,22 @@
                           personalization ; a list of 8 bytes, or nil for no personalization
                           nn ;; number of hash bytes to produce
                           )
-  (declare (xargs :guard (and (true-listp data-bytes)
-                              (all-unsigned-byte-p 8 data-bytes)
-                              ;; TODO I want to say this:
-                              ;; (< (len data-bytes) *blake2s-max-data-byte-length*)
-                              ;; But there are two potential issues related to
-                              ;; very long messages: Adding the key block can
-                              ;; make the length of d greater than expected,
-                              ;; and the expression (+ ll *bb*) in blake2s-extended-main
-                              ;; can overflow.
-                              (< (len data-bytes) (- *blake2s-max-data-byte-length* 64))
-                              (true-listp key-bytes)
+  (declare (xargs :guard (and (all-unsigned-byte-p 8 data-bytes)
+                              (true-listp data-bytes)
+                              ;; NOTE: We would like to say:
+                              ;; (<= (len data-bytes) *max-input-bytes*)
+                              ;; but that would allow potential overflows in
+                              ;; the second call of F below and in the call of
+                              ;; F in LOOP1 above.
+                              (<= (len data-bytes)
+                                  (if (= 0 (len key-bytes))
+                                      *max-input-bytes*
+                                    ;; Prevents overflows in the calls of f
+                                    ;; below:
+                                    (- *max-input-bytes* *bb*)))
                               (all-unsigned-byte-p 8 key-bytes)
-                              (<= (len key-bytes) 32)
+                              (true-listp key-bytes)
+                              (<= (len key-bytes) *max-key-bytes*)
                               (or (null salt)
                                   (and (true-listp salt)
                                        (all-unsigned-byte-p 8 salt)
@@ -182,27 +140,40 @@
                                        (all-unsigned-byte-p 8 personalization)
                                        (equal 8 (len personalization))))
                               (posp nn)
-                              (<= nn 32))))
+                              (<= nn *max-hash-bytes*))
+                  :guard-hints (("Goal" :in-theory (enable wordp natp unsigned-byte-p)))))
   (let* ((ll (len data-bytes))
          (kk (len key-bytes))
          (salt (if salt salt (repeat 8 0)))
          (personalization (if personalization personalization (repeat 8 0)))
          (parameter-block (parameter-block nn kk salt personalization))
-         (d (d-blocks data-bytes key-bytes)))
-    (blake2s-extended-main d
-                           ll
-                           kk
-                           nn
-                           parameter-block)))
+         (d (d-blocks data-bytes key-bytes))
+         (dd (len d))
+         ;; XOR in the parameter block:
+         (h (xor-words (iv) parameter-block)) ; this is what differs from the version in blake2s.lisp
+         ;; Process padded key and data blocks:
+         (h (if (> dd 1)
+                ;; The FOR loop:
+                (loop1 0 (- dd 2) h d)
+              h))
+         ;; Final block:
+         (h (if (= kk 0)
+                (f h (nth (- dd 1) d) ll t)
+              (f h
+                 (nth (- dd 1) d)
+                 (+ ll *bb*)
+                 t))))
+    ;; Extract first nn bytes to form the returned hash:
+    (take nn (words-to-bytes h))))
 
 (defthm len-of-blake2s-extended
   (implies (and (posp nn)
-                (<= nn 32))
+                (<= nn *max-hash-bytes*))
            (equal (len (blake2s-extended data-bytes key-bytes salt personalization nn))
                   nn))
   :hints (("Goal" :in-theory (enable blake2s-extended))))
 
 (defthm all-unsigned-byte-p-of-blake2s-extended
-  (implies (<= nn 32)
+  (implies (<= nn *max-hash-bytes*)
            (all-unsigned-byte-p 8 (blake2s-extended data-bytes key-bytes salt personalization nn)))
   :hints (("Goal" :in-theory (enable blake2s-extended))))
